new/proof/github_com/sanjit_bhat/pav/merkle_proof/theory.v
@@ -782,20 +782,23 @@ Fixpoint is_const_label_len t :=
   | _ => True
   end.
 
-Lemma cutless_new_put t label val :
-  is_Some (pure_put t label val) →
-  is_cutless_path t label.
+Lemma cutless_new_put t t' label val :
+  pure_put t label val = Some t' →
+  is_cutless_path t' label.
 Proof.
   autounfold with merkle.
   remember max_depth as limit. clear Heqlimit.
   remember 0%nat as depth. clear Heqdepth.
-  revert t depth.
+  revert t t' depth.
   induction limit as [? IH] using lt_wf_ind.
   intros *. rewrite pure_put_unfold.
-  destruct t; simpl; intros; try done.
-  case_match; try done.
-  case_match; try done.
-  eapply (IH n); [lia|done].
+  destruct t; simpl; intros;
+    try case_decide; try case_match; try case_match;
+    simplify_eq/=; try done.
+  - ospecialize (IH n _); [lia|].
+    repeat case_match; by eapply IH.
+  - ospecialize (IH n _); [lia|].
+    repeat case_match; by eapply IH.
 Qed.
 
 Lemma cutless_over_put t t' label0 label1 val :
